SCCGraphPlanTheoremScript.sml
@@ -10,6 +10,7 @@ open FM_planTheory
 open sublistTheory;
 open GraphPlanTheoremTheory;
 open relationTheory;
+open SCCTheory;
 val _ = new_theory "SCCGraphPlanTheorem";
 
 
@@ -19,19 +20,13 @@ val ancestors_def = Define
  `ancestors(PROB: 'a problem, vs: ('a -> bool)) = 
     {v: 'a | (?v': 'a. v' IN vs /\ ((dep_tc(PROB)) v v') ) /\ (!v': 'a. v' IN vs ==> ~((dep_tc(PROB)) v' v))}`;
 
-val dep_var_set_relaxed_def = Define
-  `dep_var_set_relaxed (PROB, vs1, vs2)
-          <=> ? v1 v2. (v1 IN vs1) /\ (v2 IN vs2) /\ dep(PROB, v1, v2)`;
-
-val scc_def = Define 
-`scc(PROB, vs) 
-    = (!v1 v2. v1 IN vs /\ v2 IN vs ==> ((dep_tc(PROB)) v1 v2) /\ ((dep_tc(PROB)) v2 v1))
-          /\ (!vs'. ~(vs'= vs) ==> ~(dep_var_set_relaxed(PROB, vs, vs')) \/ ~(dep_var_set_relaxed(PROB, vs', vs)))
-          /\ ~(vs = EMPTY) /\ (!v. v IN vs ==> ?v'. v' IN vs /\ dep(PROB, v, v'))`;
+val scc_vs_def = Define 
+`scc_vs(PROB, vs) 
+    = SCC (\v1' v2'. dep(PROB, v1', v2')) vs`;
  
 
 val scc_set_def = Define
-`scc_set(PROB, S) = !vs. vs IN S /\ ~(DISJOINT vs (FDOM(PROB.I))) ==> scc(PROB, vs)`;
+`scc_set(PROB, S) = !vs. vs IN S /\ ~(DISJOINT vs (FDOM(PROB.I))) ==> scc_vs(PROB, vs)`;
 
 
 val sum_scc_parents_def 
@@ -45,15 +40,20 @@ val childless_vs_def = Define`
 val childless_svs_def = Define`
       childless_svs(PROB, S) = !vs. vs IN S ==> (childless_vs(PROB, vs))`;
 
+val problem_scc_set_def = Define`
+      problem_scc_set(PROB) = {vs | (scc_vs(PROB, vs)) }`;
+
 
 val childless_problem_scc_set_def = Define`
-      childless_problem_scc_set(PROB) = {vs | (scc(PROB, vs)) /\ (childless_vs(PROB, vs))}`;
+      childless_problem_scc_set(PROB) = {vs | (scc_vs(PROB, vs)) /\ (childless_vs(PROB, vs))}`;
+
+
 
 val single_child_parents_def = Define
 `single_child_parents(PROB, vs) 
            = {vs' | vs' SUBSET (ancestors(PROB, vs)) 
                        /\ childless_vs(prob_proj(PROB, (FDOM PROB.I) DIFF vs), vs') 
-                            /\scc(PROB, vs')}`;
+                            /\scc_vs(PROB, vs')}`;
 
 val single_child_ancestors_def_1 = store_thm("single_child_ancestors_def_1",
 ``WF (\x y. CARD (FDOM (FST(x)).I ) < CARD(FDOM ((FST(y)).I)))``,
@@ -109,11 +109,13 @@ THEN METIS_TAC[single_child_ancestors_def_2]);
 
 val member_leaves_def = Define
      `member_leaves(PROB, S) 
-           =  (\vs. (scc(PROB, vs) /\ childless_vs(PROB, vs))) INTER S`;
+           =  (\vs. (scc_vs(PROB, vs) /\ childless_vs(PROB, vs))) INTER S`;
 
 val problem_wo_vs_ancestors_def = Define
   `problem_wo_vs_ancestors(PROB, vs) = 
               prob_proj(PROB, FDOM PROB.I DIFF (vs ∪ BIGUNION (single_child_ancestors (PROB,vs))))`;
+
+
 
 val scc_lemma_1_1 = store_thm("scc_lemma_1_1",
 ``!PROB S. FINITE(S) ==> FINITE((member_leaves(PROB, S)))``,
@@ -121,7 +123,7 @@ SRW_TAC[][member_leaves_def]
 THEN METIS_TAC[FINITE_INTER]);
 
 val scc_lemma_1_2 = store_thm("scc_lemma_1_2",
-``!PROB vs S. vs IN member_leaves(PROB, S) ==> scc(PROB, vs)``,
+``!PROB vs S. vs IN member_leaves(PROB, S) ==> scc_vs(PROB, vs)``,
 SRW_TAC[][member_leaves_def]);
 
 val scc_lemma_1_3 = store_thm("scc_lemma_1_3",
@@ -150,7 +152,7 @@ SRW_TAC[][member_leaves_def]);
 
 val scc_main_lemma_1_1_1_1_1_1 = store_thm("scc_main_lemma_1_1_1_1_1_1",
 ``!PROB v1 v2. planning_problem(PROB) /\ dep(PROB, v1, v2)
-               ==> (v1 IN FDOM(PROB.I) /\ v1 IN FDOM(PROB.I))``,
+               ==> (v1 IN FDOM(PROB.I) /\ v2 IN FDOM(PROB.I))``,
 SRW_TAC[][planning_problem_def, dep_def]
 THEN METIS_TAC[SUBSET_DEF])
 
@@ -163,40 +165,31 @@ THEN SRW_TAC[][]
 THEN METIS_TAC[scc_main_lemma_1_1_1_1_1_1])
 
 val scc_main_lemma_1_1_1_1 = store_thm("scc_main_lemma_1_1_1_1",
-``!PROB vs. planning_problem(PROB) /\ scc(PROB, vs) ==> vs SUBSET FDOM(PROB.I)``,
-SRW_TAC[][scc_def]
+``!PROB vs. planning_problem(PROB) /\ scc_vs(PROB, vs) ==> vs SUBSET FDOM(PROB.I)``,
+SRW_TAC[][scc_vs_def, SCC_def]
 THEN REWRITE_TAC[SUBSET_DEF]
-THEN METIS_TAC[scc_main_lemma_1_1_1_1_1])
+THEN METIS_TAC[scc_main_lemma_1_1_1_1_1, dep_tc_def])
 
 
 
-val scc_main_lemma_1_1_1_2_1 = store_thm("scc_main_lemma_1_1_1_2_1",
+val scc_main_lemma_x = store_thm("scc_main_lemma_x",
 ``!s t x. x IN s /\ ~(x IN t) ==> ~(s = t)``,
 METIS_TAC[])
  
-val scc_main_lemma_1_1_1_2_2 = store_thm("scc_main_lemma_1_1_1_2_2",
-``!PROB vs vs'. scc(PROB, vs) /\ scc(PROB, vs') /\ ~(vs = vs') ==> DISJOINT vs vs'``,
-SRW_TAC[][] 
-THEN SPOSE_NOT_THEN STRIP_ASSUME_TAC
-THEN FULL_SIMP_TAC(srw_ss()) [DISJOINT_DEF, INTER_DEF, GSPEC_ETA, GSYM MEMBER_NOT_EMPTY]
-THEN FULL_SIMP_TAC(bool_ss)[scc_def]
-THEN Q.PAT_ASSUM `∀vs''.
-        vs'' ≠ vs' ⇒
-        ¬dep_var_set_relaxed (PROB,vs',vs'') ∨ ¬dep_var_set_relaxed (PROB,vs'',vs')` (MP_TAC o Q.SPEC `vs`)
-THEN SRW_TAC[][]
-THEN SRW_TAC[][dep_var_set_relaxed_def]
-THEN METIS_TAC[])
+val scc_main_lemma_xx = store_thm("scc_main_lemma_1_xx",
+``!PROB vs vs'. scc_vs(PROB, vs) /\ scc_vs(PROB, vs') /\ ~(vs = vs') ==> DISJOINT vs vs'``,
+METIS_TAC[scc_disjoint_lemma, scc_vs_def])
 
 
 val scc_main_lemma_1_1_1_2 = store_thm("scc_main_lemma_1_1_1_2",
-``!PROB vs vs'. ~(DISJOINT vs vs') /\ scc(PROB, vs) /\ scc(PROB, vs') ==> (vs = vs')``,
-METIS_TAC[scc_main_lemma_1_1_1_2_2])
+``!PROB vs vs'. ~(DISJOINT vs vs') /\ scc_vs(PROB, vs) /\ scc_vs(PROB, vs') ==> (vs = vs')``,
+METIS_TAC[scc_disjoint_lemma, scc_vs_def])
 
 val scc_main_lemma_1_1_1 = store_thm("scc_main_lemma_1_1_1",
-``!PROB S vs. planning_problem(PROB) /\ FDOM(PROB.I) SUBSET BIGUNION S /\ scc_set(PROB, S) /\ scc(PROB, vs)
+``!PROB S vs. planning_problem(PROB) /\ FDOM(PROB.I) SUBSET BIGUNION S /\ scc_set(PROB, S) /\ scc_vs(PROB, vs)
               ==> vs IN S``,
 SRW_TAC[][]
-THEN `!v. v IN vs ==> ( vs IN S' (* /\ v IN vs' /\ scc(PROB, vs') /\ (vs' = vs)*))` by 
+THEN `!v. v IN vs ==> ( vs IN S' (* /\ v IN vs' /\ scc_vs(PROB, vs') /\ (vs' = vs)*))` by 
      (`vs SUBSET BIGUNION S'` by METIS_TAC[scc_main_lemma_1_1_1_1, SUBSET_TRANS]
       THEN SRW_TAC[][]
       THEN `∃vs'. vs' ∈ S' ∧ v ∈ vs'` by METIS_TAC[IN_BIGUNION, SUBSET_DEF]
@@ -206,11 +199,12 @@ THEN `!v. v IN vs ==> ( vs IN S' (* /\ v IN vs' /\ scc(PROB, vs') /\ (vs' = vs)*
       THEN MP_TAC(scc_main_lemma_1_1_1_1 |> Q.SPECL[`PROB`, `vs`])
       THEN SRW_TAC[][SUBSET_DEF]
       THEN FULL_SIMP_TAC(srw_ss())[INTER_DEF, SUBSET_DEF, GSPEC_ETA, GSYM MEMBER_NOT_EMPTY]
-      THEN `scc(PROB, vs')` by METIS_TAC[]
+      THEN `scc_vs(PROB, vs')` by METIS_TAC[]
       THEN `~(DISJOINT vs vs')` by (SRW_TAC[][DISJOINT_DEF,INTER_DEF, GSPEC_ETA, GSYM MEMBER_NOT_EMPTY]
                                   THEN Q.EXISTS_TAC `v` THEN SRW_TAC[][])
       THEN METIS_TAC[scc_main_lemma_1_1_1_2])
-THEN METIS_TAC[MEMBER_NOT_EMPTY, scc_def]);
+THEN FULL_SIMP_TAC(srw_ss())[scc_vs_def, SCC_def |> Q.SPECL [`(λv1' v2'. dep (PROB,v1',v2'))`, `vs`]]
+THEN METIS_TAC[MEMBER_NOT_EMPTY]);
  
 val scc_main_lemma_1_1 = store_thm("scc_main_lemma_1_1",
 ``!PROB S. planning_problem(PROB) /\ FDOM PROB.I SUBSET BIGUNION S /\ scc_set(PROB, S)
@@ -220,16 +214,87 @@ THEN EQ_TAC
 THEN SRW_TAC[][]
 THEN METIS_TAC[scc_main_lemma_1_1_1])
 
-val scc_main_lemma_1_2 = store_thm("scc_main_lemma_1_2",
-``!PROB. ((FDOM PROB.I = EMPTY) = (childless_problem_scc_set(PROB) = EMPTY))``,
+val scc_main_lemma_1_2_1 = store_thm("scc_main_lemma_1_2_1",
+``!PROB. planning_problem(PROB) ==> ((FDOM PROB.I = EMPTY) ==> (!vs. ~scc_vs(PROB, vs)))``,
+SRW_TAC[][]
+THEN SPOSE_NOT_THEN STRIP_ASSUME_TAC
+THEN FULL_SIMP_TAC(bool_ss)[GSYM MEMBER_NOT_EMPTY, scc_vs_def, SCC_def]
+THEN `(λv1' v2'. dep (PROB,v1',v2'))⁺ x x ∧
+ (λv1' v2'. dep (PROB,v1',v2'))⁺ x x` by SRW_TAC[][]
+THEN MP_TAC(scc_main_lemma_1_1_1_1_1 |> Q.SPECL [`PROB`, `x`, `x`])
+THEN SRW_TAC[][dep_tc_def])
+
+
+val scc_main_lemma_1_2_2_1 = store_thm("scc_main_lemma_1_2_2_1",
+``!PROB. StrongOrder(REL_RESTRICT (\vs1 vs2. dep_var_set(PROB, vs2, vs1))^+ (problem_scc_set(PROB)))``,
 cheat)
+
+val scc_main_lemma_1_2_2_2 = store_thm("scc_main_lemma_1_2_2_2",
+``!PROB. FINITE (problem_scc_set(PROB))``,
+cheat)
+
+val scc_main_lemma_1_2_2_3 = store_thm("scc_main_lemma_1_2_2_3",
+``!PROB. ~(FDOM(PROB.I) = EMPTY) /\ planning_problem(PROB) ==> ?vs. scc_vs(PROB, vs)``,
+cheat)
+
+val scc_main_lemma_1_2_2_4 = store_thm("scc_main_lemma_1_2_2_4",
+``!R s min. (!x. REL_RESTRICT (R^+) s x min ==> ~(x IN s))
+            ==> !x'. x' IN s ==> ~(R x' min)``,
+(* WF_TC_EQN *)
+cheat)
+
+
+val scc_main_lemma_1_2_2 = store_thm("scc_main_lemma_1_2_2",
+``!PROB. planning_problem(PROB) /\ ~(FDOM(PROB.I) = EMPTY) ==> ?vs. scc_vs(PROB, vs) /\ childless_vs(PROB, vs)``,
+(* SRW_TAC[][]
+THEN MP_TAC(scc_main_lemma_1_2_2_1 |> Q.SPEC `PROB`)
+THEN SRW_TAC[][]
+THEN MP_TAC(scc_main_lemma_1_2_2_2 |> Q.SPEC `PROB`)
+THEN SRW_TAC[][]
+THEN MP_TAC(FINITE_StrongOrder_WF |> Q.ISPEC `(\vs1 vs2. dep_var_set(PROB, vs2, vs1))^+`|> Q.SPEC  `(problem_scc_set(PROB))`)
+THEN SRW_TAC[][]
+THEN MP_TAC(scc_main_lemma_1_2_2_3 |> Q.SPEC `PROB`)
+THEN SRW_TAC[][]
+THEN FULL_SIMP_TAC(srw_ss())[(WF_DEF |> Q.ISPEC `(REL_RESTRICT (\vs1 vs2. dep_var_set(PROB, vs2, vs1))^+ (problem_scc_set(PROB)))`)]
+THEN `(∃w: ('a -> bool). {vs' | scc_vs (PROB,vs')} w)` by (Q.EXISTS_TAC `vs` THEN SRW_TAC[][GSPEC_ETA])
+THEN Q.PAT_ASSUM `!x. P x` (MP_TAC o Q.SPEC `{vs' | scc_vs(PROB, vs')}`)
+THEN SRW_TAC[][]
+THEN `∃min.
+        {vs' | scc_vs (PROB,vs')} min ∧
+        ∀b.
+          REL_RESTRICT (λvs1 vs2. dep_var_set (PROB,vs2,vs1))⁺
+            (problem_scc_set PROB) b min ⇒
+          ¬{vs' | scc_vs (PROB,vs')} b` by METIS_TAC[]
+THEN FULL_SIMP_TAC(srw_ss()) [GSYM problem_scc_set_def]
+THEN MP_TAC(scc_main_lemma_1_2_2_4 |> Q.ISPEC `(λvs1 vs2. dep_var_set (PROB,vs2,vs1))` |> Q.SPEC `problem_scc_set(PROB)`|> Q.SPEC  `min`)
+THEN SRW_TAC[][IN_DEF] *)
+cheat)
+
+
+val scc_main_lemma_1_2 = store_thm("scc_main_lemma_1_2",
+``!PROB. planning_problem(PROB) ==> ((FDOM PROB.I = EMPTY) = (childless_problem_scc_set(PROB) = EMPTY))``,
+SRW_TAC[][]
+THEN EQ_TAC
+THENL
+[
+   SRW_TAC[][]
+   THEN REWRITE_TAC[IN_DEF, EXTENSION,childless_problem_scc_set_def]
+   THEN SRW_TAC[][GSPEC_ETA]
+   THEN METIS_TAC[scc_main_lemma_1_2_1]
+   ,
+   FULL_SIMP_TAC(bool_ss)[childless_problem_scc_set_def, EXTENSION, GSPEC_ETA, EMPTY_DEF]
+   THEN SRW_TAC[][]
+   THEN SPOSE_NOT_THEN STRIP_ASSUME_TAC
+   THEN METIS_TAC[scc_main_lemma_1_2_2, MEMBER_NOT_EMPTY]
+])
 
 val scc_main_lemma_1_3 = store_thm("scc_main_lemma_1_3",
 ``!PROB S S'. scc_set(PROB, S) /\ S' SUBSET S ==> scc_set(prob_proj(PROB, FDOM(PROB.I) DIFF BIGUNION S'), S)``,
 cheat)
 
 val scc_main_lemma_1_4 = store_thm("scc_main_lemma_1_4",
-``!PROB vs S. scc_set(PROB, S) /\ scc(PROB, vs) /\ FDOM(PROB.I) SUBSET BIGUNION S ==> single_child_ancestors(PROB, vs) SUBSET S``,
+``!PROB vs S. scc_set(PROB, S) /\ scc_vs(PROB, vs) /\ FDOM(PROB.I) SUBSET BIGUNION S 
+              ==> single_child_ancestors(PROB, vs) SUBSET S``,
 cheat)
 
 val scc_main_lemma_1_5 = store_thm("scc_main_lemma_1_5",
@@ -244,7 +309,7 @@ val scc_main_lemma_1_6 = store_thm("scc_main_lemma_1_6",
 cheat)
 
 val scc_main_lemma_1_7 = store_thm("scc_main_lemma_1_7",
-``!PROB vs. childless_vs(PROB, vs) /\ scc(PROB, vs)
+``!PROB vs. childless_vs(PROB, vs) /\ scc_vs(PROB, vs)
             ==> problem_plan_bound(PROB)
                    <= problem_plan_bound(problem_wo_vs_ancestors(PROB, vs))
                            + problem_plan_bound(prob_proj(PROB, vs UNION (ancestors (PROB,vs))))``,
